BananasStatics.thy
@@ -92,15 +92,17 @@ inductive_cases [elim]: "\<Gamma> \<turnstile> InjV f v : t"
 
 inductive typecheck\<^sub>c\<^sub>e :: "static_environment \<Rightarrow> funct \<Rightarrow> (name \<times> name list) list \<Rightarrow> 
     (name \<rightharpoonup> type \<times> type) \<Rightarrow> bool" where
-  "typecheck\<^sub>c\<^sub>e \<Gamma> F [] Map.empty" 
-| "typecheck\<^sub>c\<^sub>e \<Gamma> F cts \<Gamma>\<^sub>e \<Longrightarrow> those (map (map_option \<mu> o var\<^sub>t_type \<Gamma>) ts) = Some ts' \<Longrightarrow> 
-    typecheck\<^sub>c\<^sub>e \<Gamma> F ((x, ts) # cts) (\<Gamma>\<^sub>e(x \<mapsto> (foldr (op \<otimes>) ts' \<one>, \<mu> F)))"
+  tcce_nil [simp]: "typecheck\<^sub>c\<^sub>e \<Gamma> F [] Map.empty" 
+| tcce_cons [simp]: "typecheck\<^sub>c\<^sub>e \<Gamma> F cts \<Gamma>\<^sub>e \<Longrightarrow> 
+    those (map (map_option \<mu> o var\<^sub>t_type \<Gamma>) ts) = Some ts' \<Longrightarrow> 
+      typecheck\<^sub>c\<^sub>e \<Gamma> F ((x, ts) # cts) (\<Gamma>\<^sub>e(x \<mapsto> (foldr (op \<otimes>) ts' \<one>, \<mu> F)))"
 
 inductive typecheck\<^sub>c\<^sub>v :: "static_environment \<Rightarrow> funct \<Rightarrow> (name \<times> name list) list \<Rightarrow> 
     (name \<rightharpoonup> type list \<times> type) \<Rightarrow> bool" where
-    "typecheck\<^sub>c\<^sub>v \<Gamma> F ((x, ts) # cts) Map.empty"
-| "typecheck\<^sub>c\<^sub>v \<Gamma> F cts \<Gamma>\<^sub>v \<Longrightarrow> those (map (map_option \<mu> o var\<^sub>t_type \<Gamma>) ts) = Some ts' \<Longrightarrow> 
-    typecheck\<^sub>c\<^sub>v \<Gamma> F ((x, ts) # cts) (\<Gamma>\<^sub>v(x \<mapsto> (ts', \<mu> F)))"
+  tccv_nil [simp]: "typecheck\<^sub>c\<^sub>v \<Gamma> F [] Map.empty"
+| tccv_cons [simp]: "typecheck\<^sub>c\<^sub>v \<Gamma> F cts \<Gamma>\<^sub>v \<Longrightarrow> 
+    those (map (map_option \<mu> o var\<^sub>t_type \<Gamma>) ts) = Some ts' \<Longrightarrow> 
+      typecheck\<^sub>c\<^sub>v \<Gamma> F ((x, ts) # cts) (\<Gamma>\<^sub>v(x \<mapsto> (ts', \<mu> F)))"
 
 fun typecheck\<^sub>c\<^sub>t_arg :: "static_environment \<Rightarrow> name \<Rightarrow> name \<Rightarrow> funct option" where
   "typecheck\<^sub>c\<^sub>t_arg \<Gamma> tn t = (if t = tn then Some Id else map_option (K o \<mu>) (var\<^sub>t_type \<Gamma> t))"
@@ -116,10 +118,9 @@ definition typecheck\<^sub>c\<^sub>t\<^sub>s :: "static_environment \<Rightarrow
 
 inductive typecheck\<^sub>d\<^sub>t :: "static_environment \<Rightarrow> name \<Rightarrow> (name \<times> name list) list \<Rightarrow> 
     static_environment \<Rightarrow> bool" where
-  "typecheck\<^sub>c\<^sub>t\<^sub>s \<Gamma> n cts = Some F \<Longrightarrow> typecheck\<^sub>c\<^sub>e \<Gamma> F cts \<Gamma>\<^sub>e \<Longrightarrow> typecheck\<^sub>c\<^sub>v \<Gamma> F cts \<Gamma>\<^sub>v \<Longrightarrow>
-      typecheck\<^sub>d\<^sub>t \<Gamma> n cts \<lparr> var\<^sub>e_type = \<Gamma>\<^sub>e, 
-                            var\<^sub>v_type = \<Gamma>\<^sub>v, 
-                            var\<^sub>t_type = [n \<mapsto> F] \<rparr>"
+  tcdt [simp]: "typecheck\<^sub>c\<^sub>t\<^sub>s \<Gamma> n cts = Some F \<Longrightarrow> typecheck\<^sub>c\<^sub>e \<Gamma> F cts \<Gamma>\<^sub>e \<Longrightarrow> 
+    typecheck\<^sub>c\<^sub>v \<Gamma> F cts \<Gamma>\<^sub>v \<Longrightarrow> 
+      typecheck\<^sub>d\<^sub>t \<Gamma> n cts \<lparr> var\<^sub>e_type = \<Gamma>\<^sub>e, var\<^sub>v_type = \<Gamma>\<^sub>v, var\<^sub>t_type = [n \<mapsto> F] \<rparr>"
 
 inductive typecheck_decl :: "static_environment \<Rightarrow> decl \<Rightarrow> static_environment \<Rightarrow> bool" 
     (infix "\<Turnstile> _ :" 60) where
@@ -134,16 +135,97 @@ inductive_cases [elim]: "\<Gamma> \<Turnstile> ExprDecl x e : \<Gamma>'"
 inductive typecheck_decls :: "static_environment \<Rightarrow> decl list \<Rightarrow> static_environment \<Rightarrow> bool" 
     (infix "\<Turnstile> _ ::" 60) where
   tcd_nil [simp]: "\<Gamma> \<Turnstile> [] :: \<Gamma>"
-| tcd_cons [simp]: "\<Gamma> \<Turnstile> \<delta> : \<Gamma>' \<Longrightarrow> binders\<^sub>d \<delta> \<inter> domain\<^sub>s \<Gamma> = {} \<Longrightarrow> \<Gamma>' \<Turnstile> \<Lambda> :: \<Gamma>'' \<Longrightarrow> 
-    \<Gamma> \<Turnstile> \<delta> # \<Lambda> :: \<Gamma>''"
+| tcd_cons [simp]: "\<Gamma> \<Turnstile> \<delta> : \<Gamma>' \<Longrightarrow> binders\<^sub>d \<delta> \<inter> domain\<^sub>s \<Gamma> = {} \<Longrightarrow> \<Gamma>' \<Turnstile> \<Delta> :: \<Gamma>'' \<Longrightarrow> 
+    \<Gamma> \<Turnstile> \<delta> # \<Delta> :: \<Gamma>''"
 
 inductive_cases [elim]: "\<Gamma> \<Turnstile> [] :: \<Gamma>'"
 inductive_cases [elim]: "\<Gamma> \<Turnstile> \<delta> # \<Lambda> :: \<Gamma>'"
 
-inductive typecheck_prog :: "prog \<Rightarrow> static_environment \<Rightarrow> type \<Rightarrow> bool" (infix "\<TTurnstile> _ \<rightarrow> " 60) where
-  tcp_prog [simp]: "empty_static \<Turnstile> \<Lambda> :: \<Gamma> \<Longrightarrow> \<Gamma> \<turnstile> e : t\<^sub>1 \<rightarrow> t\<^sub>2 \<Longrightarrow> \<Gamma> \<turnstile> v : t\<^sub>1 \<Longrightarrow> 
-    Prog \<Lambda> e v \<TTurnstile> \<Gamma> \<rightarrow> t\<^sub>2"
+inductive typecheck_prog :: "prog \<Rightarrow> static_environment \<Rightarrow> type \<Rightarrow> bool" (infix "\<TTurnstile> _ \<rightarrow>" 60) where
+  tcp_prog [simp]: "empty_static \<Turnstile> \<Delta> :: \<Gamma> \<Longrightarrow> \<Gamma> \<turnstile> e : t\<^sub>1 \<rightarrow> t\<^sub>2 \<Longrightarrow> \<Gamma> \<turnstile> v : t\<^sub>1 \<Longrightarrow> 
+    Prog \<Delta> e v \<TTurnstile> \<Gamma> \<rightarrow> t\<^sub>2"
 
-inductive_cases [elim]: "Prog \<Lambda> e v \<TTurnstile> \<Gamma>  \<rightarrow> t"
+inductive_cases [elim]: "Prog \<Delta> e v \<TTurnstile> \<Gamma> \<rightarrow> t"
+
+(* useful properties *)
+
+lemma [simp]: "var\<^sub>e_type (extend\<^sub>e\<^sub>s x (t\<^sub>1, t\<^sub>2) \<Gamma>) = (var\<^sub>e_type \<Gamma>)(x \<mapsto> (t\<^sub>1, t\<^sub>2))"
+  by (simp add: extend\<^sub>e\<^sub>s_def)
+
+lemma [simp]: "var\<^sub>v_type (extend\<^sub>e\<^sub>s x (t\<^sub>1, t\<^sub>2) \<Gamma>) = var\<^sub>v_type \<Gamma>"
+  by (simp add: extend\<^sub>e\<^sub>s_def)
+
+lemma [simp]: "var\<^sub>t_type (extend\<^sub>e\<^sub>s x (t\<^sub>1, t\<^sub>2) \<Gamma>) = var\<^sub>t_type \<Gamma>"
+  by (simp add: extend\<^sub>e\<^sub>s_def)
+
+lemma [simp]: "var\<^sub>v_type (extend\<^sub>v\<^sub>s x t \<Gamma>) = (var\<^sub>v_type \<Gamma>)(x \<mapsto> t)"
+  by (simp add: extend\<^sub>v\<^sub>s_def)
+
+lemma [simp]: "var\<^sub>e_type (extend\<^sub>v\<^sub>s x t \<Gamma>) = var\<^sub>e_type \<Gamma>"
+  by (simp add: extend\<^sub>v\<^sub>s_def)
+
+lemma [simp]: "var\<^sub>t_type (extend\<^sub>v\<^sub>s x t \<Gamma>) = var\<^sub>t_type \<Gamma>"
+  by (simp add: extend\<^sub>v\<^sub>s_def)
+
+lemma [simp]: "\<Gamma> \<turnstile> e : t\<^sub>1 \<rightarrow> t\<^sub>2 \<Longrightarrow> x \<notin> domain\<^sub>s \<Gamma> \<Longrightarrow> extend\<^sub>e\<^sub>s x (t\<^sub>1', t\<^sub>2') \<Gamma> \<turnstile> e : t\<^sub>1 \<rightarrow> t\<^sub>2"
+  and [simp]: "\<Gamma> \<turnstile> v : t \<Longrightarrow> x \<notin> domain\<^sub>s \<Gamma> \<Longrightarrow> extend\<^sub>e\<^sub>s x (t\<^sub>1', t\<^sub>2') \<Gamma> \<turnstile> v : t"
+  proof (induction \<Gamma> e t\<^sub>1 t\<^sub>2 and \<Gamma> v t rule: typecheck\<^sub>e_typecheck\<^sub>v.inducts) 
+  case (tc_var \<Gamma> y t\<^sub>1 t\<^sub>2)
+    moreover hence "x \<noteq> y" by (auto simp add: domain\<^sub>s_def)
+    ultimately show ?case by simp
+  qed (simp_all add: extend\<^sub>e\<^sub>s_def)
+
+lemma [simp]: "\<Gamma> \<turnstile> e : t\<^sub>1 \<rightarrow> t\<^sub>2 \<Longrightarrow> x \<notin> domain\<^sub>s \<Gamma> \<Longrightarrow> extend\<^sub>v\<^sub>s x t' \<Gamma> \<turnstile> e : t\<^sub>1 \<rightarrow> t\<^sub>2"
+  and [simp]: "\<Gamma> \<turnstile> v : t \<Longrightarrow> x \<notin> domain\<^sub>s \<Gamma> \<Longrightarrow> extend\<^sub>v\<^sub>s x t' \<Gamma> \<turnstile> v : t"
+  by (induction \<Gamma> e t\<^sub>1 t\<^sub>2 and \<Gamma> v t rule: typecheck\<^sub>e_typecheck\<^sub>v.inducts) simp_all
+
+(* static uniqueness *)
+
+(* not actually true! fix once we have polymorphism *)
+lemma unique_typechecking\<^sub>e [elim]: "\<Gamma> \<turnstile> e : t\<^sub>1 \<rightarrow> t\<^sub>2 \<Longrightarrow> \<Gamma> \<turnstile> e : t\<^sub>1' \<rightarrow> t\<^sub>2' \<Longrightarrow> t\<^sub>1 = t\<^sub>1' \<and> t\<^sub>2 = t\<^sub>2'"
+  and unique_typechecking\<^sub>v [elim]: "\<Gamma> \<turnstile> v : t \<Longrightarrow> \<Gamma> \<turnstile> v : t' \<Longrightarrow> t = t'"
+  by (induction \<Gamma> e t\<^sub>1 t\<^sub>2 and \<Gamma> v t rule: typecheck\<^sub>e_typecheck\<^sub>v.inducts) simp_all
+
+lemma unique_typechecking\<^sub>c\<^sub>e [elim]: "typecheck\<^sub>c\<^sub>e \<Gamma> F cts \<Gamma>\<^sub>e \<Longrightarrow> typecheck\<^sub>c\<^sub>e \<Gamma> F cts \<Gamma>\<^sub>e' \<Longrightarrow> \<Gamma>\<^sub>e = \<Gamma>\<^sub>e'"
+  proof (induction \<Gamma> F cts \<Gamma>\<^sub>e arbitrary: \<Gamma>\<^sub>e' rule: typecheck\<^sub>c\<^sub>e.induct)
+  case (tcce_nil \<Gamma> F)
+    thus ?case 
+      by (induction \<Gamma> F "[]::(name \<times> name list) list" \<Gamma>\<^sub>e' rule: typecheck\<^sub>c\<^sub>e.induct) simp_all
+  next case (tcce_cons \<Gamma> F cts \<Gamma>\<^sub>e ts ts' x)
+    with tcce_cons(4) show ?case 
+      by (induction \<Gamma> F "(x, ts) # cts" \<Gamma>\<^sub>e' rule: typecheck\<^sub>c\<^sub>e.induct) simp_all
+  qed
+
+lemma unique_typechecking\<^sub>c\<^sub>v [elim]: "typecheck\<^sub>c\<^sub>v \<Gamma> F cts \<Gamma>\<^sub>v \<Longrightarrow> typecheck\<^sub>c\<^sub>v \<Gamma> F cts \<Gamma>\<^sub>v' \<Longrightarrow> \<Gamma>\<^sub>v = \<Gamma>\<^sub>v'"
+  proof (induction \<Gamma> F cts \<Gamma>\<^sub>v arbitrary: \<Gamma>\<^sub>v' rule: typecheck\<^sub>c\<^sub>v.induct)
+  case (tccv_nil \<Gamma> F)
+    thus ?case 
+      by (induction \<Gamma> F "[]::(name \<times> name list) list" \<Gamma>\<^sub>v' rule: typecheck\<^sub>c\<^sub>v.induct) simp_all
+  next case (tccv_cons \<Gamma> F cts \<Gamma>\<^sub>v ts ts' x)
+    with tccv_cons(4) show ?case 
+      by (induction \<Gamma> F "(x, ts) # cts" \<Gamma>\<^sub>v' rule: typecheck\<^sub>c\<^sub>v.induct) simp_all
+  qed
+
+lemma unique_typechecking\<^sub>d\<^sub>t [elim]: "typecheck\<^sub>d\<^sub>t \<Gamma> x cts \<Gamma>' \<Longrightarrow> typecheck\<^sub>d\<^sub>t \<Gamma> x cts \<Gamma>'' \<Longrightarrow> \<Gamma>' = \<Gamma>''"
+  proof (induction \<Gamma> x cts \<Gamma>' rule: typecheck\<^sub>d\<^sub>t.induct)
+  case (tcdt \<Gamma> x cts F \<Gamma>\<^sub>e \<Gamma>\<^sub>v)
+    with tcdt(4) show ?case
+      by (induction \<Gamma> x cts \<Gamma>'' rule: typecheck\<^sub>d\<^sub>t.induct)
+         (simp, metis unique_typechecking\<^sub>c\<^sub>e unique_typechecking\<^sub>c\<^sub>v)
+  qed
+
+lemma [elim]: "\<Gamma> \<Turnstile> \<delta> : \<Gamma>' \<Longrightarrow> \<Gamma> \<Turnstile> \<delta> : \<Gamma>'' \<Longrightarrow> \<Gamma>' = \<Gamma>''"
+  proof (induction \<Gamma> \<delta> \<Gamma>' rule: typecheck_decl.induct)
+  case (tcd_expr \<Gamma> e t\<^sub>1 t\<^sub>2 x)
+    with tcd_expr(2) show ?case 
+      by (induction \<Gamma> "ExprDecl x e" \<Gamma>'' rule: typecheck_decl.induct) (metis unique_typechecking\<^sub>e)
+  next case (tcd_val \<Gamma> v t x)
+    with tcd_val(2) show ?case
+      by (induction \<Gamma> "ValDecl x v" \<Gamma>'' rule: typecheck_decl.induct) (metis unique_typechecking\<^sub>v)
+  next case (tcd_type \<Gamma> x cts \<Gamma>')
+    with tcd_type(2) show ?case
+      by (induction \<Gamma> "TypeDecl x cts" \<Gamma>'' rule: typecheck_decl.induct) 
+         (metis unique_typechecking\<^sub>d\<^sub>t)
+  qed
 
 end
